% author: Shuning Zhang
% creation date: 2019-12-20
\documentclass[a4paper, 11pt]{ctexart}
\usepackage[top=2cm, bottom=2cm, left=2.5cm, right=2.5cm]{geometry}
\usepackage{amsmath, amssymb}   
\newcommand{\re}{\mathrm{Re}\,}
\newcommand{\im}{\mathrm{Im}\,}
\begin{document}
\pagestyle{empty}
\begin{enumerate}
    \item % 1
        略.
    \item % 2
        {\heiti 证明}\quad 设 $z = x + iy$.
        \begin{enumerate}
            \item % a
                $\re(iz) = \re(ix - y) = \re(-y + ix) = -y = -\im(x + iy) = -\im z$;
            \item % b
                $\im(iz) = \im(ix - y) = \im(-y + ix) = x = \re(x + iy) = \re z$.
        \end{enumerate}
    \item % 3
        {\heiti 证明}\quad 设 $z = x + iy$. 对 $(1 + z)^2$, 有
        \begin{align*}
            (1 + z)^2 &= ((1+x) + (0+iy))^2 \\
                      &= (x+1)^2 + 2(x+1)iy + i^2y^2 \\
                      &= (x^2 + 2x + 1) + (2ixy + 2iy) - y^2.
        \end{align*}
        对 $1 + 2z + z^2$, 有
        \begin{align*}
            1 + 2z + z^2 &= 1 + 2(x + iy) + (x + iy)^2 \\
                         &= 1 + (2x + 2iy) + (x^2 + 2ixy + i^2y^2) \\
                         &= (x^2 + 2x + 1) + (2ixy + 2iy) - y^2.
        \end{align*}
        因此, $(1 + z)^2 = 1 + 2z + z^2$.
    \item % 4
        略.
    \item % 5
        略.
    \item % 6
        略.
    \item % 7
        略.
    \item 8
    \item 9
    \item 10
\end{enumerate}
\end{document}