% % @author Shuning Zhang
% % @date 2020.2.18
% \documentclass[a4paper, 11pt]{article}
% \usepackage{amsfonts, amsmath, amssymb, amsthm}
% \usepackage{color}
% % \usepackage{ctex}
% \usepackage{enumerate}
% \usepackage[bottom=2cm, left=2.5cm, right=2.5cm, top=2cm]{geometry}
% \usepackage{multicol}
% \newcommand{\Arg}{\mathrm{Arg}\,}
% \newcommand{\im}{\mathrm{Im}\,}
% \newcommand{\re}{\mathrm{Re}\,}
% \begin{document}
\begin{enumerate}
    \item % 1
        \begin{multicols}{2}
            \begin{enumerate}
                \item % a
                    $z \neq \pm1$;
                \item % b
                    $z \neq 0$;
                \item % c
                    $\re{z} \neq 0$;
                \item % d
                    $(\re{z})^2 + (\im{z})^2 \neq 1$.
            \end{enumerate}
        \end{multicols}
    \item % 2
        \begin{align*}
            f(z) &= z^3 + z + 1 \\
            &= (x+iy)^3 + (x+iy) + 1 \\
            &= x^3 + i3x^2y - 3xy^3 - iy^3 + x + iy + 1 \\
            &= (x^3 - 3xy^3 + x + 1) + i(3x^2y - y^3 + y).   
        \end{align*}
        Hence
        \begin{gather*}
            u(x, y) = x^3 - 3xy^3 + x + 1, \\
            v(x, y) = 3x^2y - y^3 + y.
        \end{gather*}
    \item % 3
        $\overline{z}^2 + 2iz$.
    \item % 4
        $(r + 1/r)\cos\theta + i(r - 1/r)\sin\theta$.
\end{enumerate}
% \end{document}
        