% author: Shuning Zhang
% creation date: 2019-12-20
\documentclass[a4paper, 11pt]{ctexart}
\usepackage[top=2cm, bottom=2cm, left=2.5cm, right=2.5cm]{geometry}
\usepackage{amsmath, amssymb}   
\newcommand{\re}{\mathrm{Re}\,}
\newcommand{\im}{\mathrm{Im}\,}
\begin{document}
\pagestyle{empty}
\begin{enumerate}
    \item % 1
    \item % 2 
    \item % 3
    \item % 4
    \item % 5
    \item % 6
    \item % 7
    \item % 8
    \item % 9
    \item % 10
    \item % 11
    \item % 12
    \item % 13
    \item % 14
    \item % 15
        {\heiti 证明}\quad 令 $z = x + iy$, $\bar z = x - iy$, 那么 $\re z = \dfrac{z + \bar z}{2}$, $\im z = \dfrac{z - \bar z}{2i}$. 对 $x^2 - y^2 = 1$, 有
        \begin{align*}
            x^2 - y^2 - 1 &= (\re z)^2 - (\im z)^2 - 1 \\
                          &= \frac{(z + \bar z)^2}{4} + \frac{(z - \bar z)^2}{4} - 1 \\
                          &= \frac{z^2 + \bar z^2}{2} - 1 = 0,     
        \end{align*}
        即 $z^2 + \bar z^2 = 2$.
    \item % 16
\end{enumerate}
\end{document}